src/Goose/GoZeroValues.v
@@ -6,12 +6,13 @@ Arguments zeroValue T {_}.
 
 Instance uint64_zero : HasGoZero uint64 := 0.
 Instance bool_zero : HasGoZero bool := false.
-
-Axiom byte0 : byte.
-Instance byte_zero : HasGoZero byte := byte0.
-
-Instance ptr_zero ty : HasGoZero (Ptr.t ty) := nullptr _.
-Instance file_zero : HasGoZero File := nilFile.
-Instance slice_zero T : HasGoZero (slice.t T) := slice.nil _.
-
 Instance string_zero : HasGoZero string := ""%string.
+
+Section GoModel.
+  Context `{GoModel}.
+  Global Instance byte_zero : HasGoZero byte := byte0.
+
+  Global Instance ptr_zero ty : HasGoZero (Ptr ty) := nullptr _.
+  Global Instance file_zero : HasGoZero File := nilFile.
+  Global Instance slice_zero T : HasGoZero (slice.t T) := slice.nil _.
+End GoModel.
